Be careful with argument order and superclasses.

prototype/Is/LeftModule.v
@@ -5,14 +5,15 @@ From Maniunfold.Is Require Export
 
 Import AdditiveNotations.
 
-Class IsLeftModule {S A : Type} {S_has_eqv : HasEqv S}
-  (S_has_add : HasAdd S) (S_has_zero : HasZero S) (S_has_neg : HasNeg S)
-  (S_has_mul : HasMul S) (S_has_one : HasOne S) {A_has_eqv : HasEqv A}
+Class IsLeftModule {A S : Type} {A_has_eqv : HasEqv A}
   (A_has_opr : HasOpr A) (A_has_idn : HasIdn A) (A_has_inv : HasInv A)
+  {S_has_eqv : HasEqv S}
+  (S_has_add : HasAdd S) (S_has_zero : HasZero S) (S_has_neg : HasNeg S)
+  (S_has_mul : HasMul S) (S_has_one : HasOne S)
   (has_lsmul : HasLSMul S A) : Prop := {
   lsmul_is_proper :> IsProper (eqv ==> eqv ==> eqv) lsmul;
   add_zero_neg_mul_one_is_ring :> IsRing add zero neg mul one;
-  opr_idn_inv_is_abelian_group :> IsAbelianGroup opr idn inv;
+  opr_idn_inv_is_abelian_group :> IsAbelianGroup (A := A) opr idn inv;
   left_biidentifiable : forall x : A, 1 <* x == x;
   left_bicompatible : forall (a b : S) (x : A),
     (a * b) <* x == a <* (b <* x);
