prototype/Has/Distance.v
@@ -1,6 +1,6 @@
 From Maniunfold Require Export
   Init.
 
-Class HasDist (S A : Type) : Type := dist : A -> A -> S.
+Class HasDist (A S : Type) : Type := dist : A -> A -> S.
 
 Typeclasses Transparent HasDist.
