prototype/Is/Bimodule.v
@@ -3,16 +3,18 @@ From Maniunfold.Has Require Export
 From Maniunfold.Is Require Export
   LeftModule RightModule Heteroassociative.
 
-Class IsBimodule {LS RS A : Type} {LS_has_eqv : HasEqv LS}
-  (LS_has_add : HasAdd LS) (LS_has_zero : HasZero LS) (LS_has_neg : HasNeg LS)
-  (LS_has_mul : HasMul LS) (LS_has_one : HasOne LS) {RS_has_eqv : HasEqv RS}
-  (RS_has_add : HasAdd RS) (RS_has_zero : HasZero RS) (RS_has_neg : HasNeg RS)
-  (RS_has_mul : HasMul RS) (RS_has_one : HasOne RS) {A_has_eqv : HasEqv A}
+Class IsBimodule {A LS RS : Type} {A_has_eqv : HasEqv A}
   (A_has_opr : HasOpr A) (A_has_idn : HasIdn A) (A_has_inv : HasInv A)
+  {LS_has_eqv : HasEqv LS}
+  (LS_has_add : HasAdd LS) (LS_has_zero : HasZero LS) (LS_has_neg : HasNeg LS)
+  (LS_has_mul : HasMul LS) (LS_has_one : HasOne LS)
+  {RS_has_eqv : HasEqv RS}
+  (RS_has_add : HasAdd RS) (RS_has_zero : HasZero RS) (RS_has_neg : HasNeg RS)
+  (RS_has_mul : HasMul RS) (RS_has_one : HasOne RS)
   (has_lsmul : HasLSMul LS A) (has_rsmul : HasRSMul RS A) : Prop := {
-  add_zero_neg_mul_one_opr_idn_inv_lsmul_is_left_module :>
-    IsLeftModule add zero neg mul one opr idn inv lsmul;
-  add_zero_neg_mul_one_opr_idn_inv_rsmul_is_right_module :>
-    IsRightModule add zero neg mul one opr idn inv rsmul;
+  opr_idn_inv_add_zero_neg_mul_one_lsmul_is_left_module :>
+    IsLeftModule opr idn inv add zero neg mul one lsmul;
+  opr_idn_inv_add_zero_neg_mul_one_rsmul_is_right_module :>
+    IsRightModule opr idn inv add zero neg mul one rsmul;
   lsmul_rsmul_is_heteroassociative : IsHeteroassociative lsmul rsmul;
 }.
