prototype/Is/FreeLeftModule.v
@@ -8,16 +8,17 @@ From Maniunfold.Is Require Export
 (** TODO Investigate whether the use of
     a nonconstructive existential quantifier is dubious. *)
 
-Class IsFreeLeftModule {I S A : Type}
-  {I_has_eqv : HasEqv I} {I_has_enum : HasEnum I} {S_has_eqv : HasEqv S}
-  (S_has_add : HasAdd S) (S_has_zero : HasZero S) (S_has_neg : HasNeg S)
-  (S_has_mul : HasMul S) (S_has_one : HasOne S) {A_has_eqv : HasEqv A}
+Class IsFreeLeftModule {A S I : Type} {A_has_eqv : HasEqv A}
   (A_has_opr : HasOpr A) (A_has_idn : HasIdn A) (A_has_inv : HasInv A)
-  (has_lsmul : HasLSMul S A) (has_basis : HasBasis I A) : Prop := {
+  {S_has_eqv : HasEqv S} (S_has_add : HasAdd S) (S_has_zero : HasZero S)
+  (S_has_neg : HasNeg S) (S_has_mul : HasMul S) (S_has_one : HasOne S)
+  (has_lsmul : HasLSMul S A)
+  {I_has_eqv : HasEqv I} {I_has_enum : HasEnum I}
+  (has_basis : HasBasis I A) : Prop := {
   basis_is_proper :> IsProper (eqv ==> eqv) basis;
   I_is_finite :> IsFinite I;
-  add_zero_neg_mul_one_opr_idn_inv_lsmul_is_left_module :>
-    IsLeftModule add zero neg mul one opr idn inv lsmul;
+  opr_idn_inv_add_zero_neg_mul_one_lsmul_is_left_module :>
+    IsLeftModule opr idn inv add zero neg mul one lsmul;
   spanning : forall x : A, exists coeffs : I -> S,
     let terms (i : I) := coeffs i <* basis i in
     fold_right opr idn (map terms enum) == x;
