prototype/Is/Heterocommutative.v
@@ -3,8 +3,8 @@ From Maniunfold.Has Require Export
 From Maniunfold.Is Require Export
   Setoid.
 
-Class IsHeterocommutative {S A : Type} {has_eqv : HasEqv S}
-  (has_dist : HasDist S A) : Prop := {
+Class IsHeterocommutative {A B : Type} {has_eqv : HasEqv B}
+  (has_dist : HasDist A B) : Prop := {
   eqv_is_setoid :> IsSetoid eqv;
   heterocommutative : forall x y : A, dist x y == dist y x;
 }.
