prototype/Is/HomogeneousBimodule.v
@@ -3,12 +3,11 @@ From Maniunfold.Has Require Export
 From Maniunfold.Is Require Export
   Bimodule.
 
-Class IsHomogeneousBimodule {S A : Type} {S_has_eqv : HasEqv S}
+Class IsHomogeneousBimodule {A S : Type} {S_has_eqv : HasEqv S}
   (S_has_add : HasAdd S) (S_has_zero : HasZero S) (S_has_neg : HasNeg S)
   (S_has_mul : HasMul S) (S_has_one : HasOne S) {A_has_eqv : HasEqv A}
   (A_has_opr : HasOpr A) (A_has_idn : HasIdn A) (A_has_inv : HasInv A)
   (has_lsmul : HasLSMul S A) (has_rsmul : HasRSMul S A) : Prop := {
-  add_zero_neg_mul_one_add_zero_neg_mul_one_opr_idn_inv_lsmul_lsmul_is_bimodule :>
-    IsBimodule add zero neg mul one add zero neg mul one
-    opr idn inv lsmul lsmul;
+  opr_idn_inv_add_zero_neg_mul_one_add_zero_neg_mul_one_lsmul_lsmul_is_bimodule :>
+    IsBimodule opr idn inv add zero neg mul one add zero neg mul one lsmul lsmul;
 }.
