prototype/Is/RightModule.v
@@ -5,14 +5,15 @@ From Maniunfold.Is Require Export
 
 Import AdditiveNotations.
 
-Class IsRightModule {S A : Type} {S_has_eqv : HasEqv S}
-  (S_has_add : HasAdd S) (S_has_zero : HasZero S) (S_has_neg : HasNeg S)
-  (S_has_mul : HasMul S) (S_has_one : HasOne S) {A_has_eqv : HasEqv A}
+Class IsRightModule {A S : Type} {A_has_eqv : HasEqv A}
   (A_has_opr : HasOpr A) (A_has_idn : HasIdn A) (A_has_inv : HasInv A)
+  {S_has_eqv : HasEqv S}
+  (S_has_add : HasAdd S) (S_has_zero : HasZero S) (S_has_neg : HasNeg S)
+  (S_has_mul : HasMul S) (S_has_one : HasOne S)
   (has_rsmul : HasRSMul S A) : Prop := {
   rsmul_is_proper :> IsProper (eqv ==> eqv ==> eqv) rsmul;
   add_zero_neg_mul_one_is_ring :> IsRing add zero neg mul one;
-  opr_idn_inv_is_abelian_group :> IsAbelianGroup opr idn inv;
+  opr_idn_inv_is_abelian_group :> IsAbelianGroup (A := A) opr idn inv;
   right_biidentity : forall x : A, x *> 1 == x;
   right_bicompatible : forall (a b : S) (x : A),
     x *> (a * b) == (x *> a) *> b;
